Add preliminary verification of intervals

shuffle.v
@@ -1,37 +1,620 @@
 Set Implicit Arguments.
 
 Require Import Coq.Lists.List.
-Require Export MSetInterface OrdersFacts OrdersLists.
+Require Import Coq.Lists.SetoidList.
 
-Require Import Coq.MSets.MSetFacts Coq.MSets.MSetProperties.
+Require MSetInterface OrdersFacts OrdersLists.
+Require Coq.MSets.MSetFacts Coq.MSets.MSetProperties.
+Require Coq.FSets.FMapInterface Coq.FSets.FMapFacts.
+
+Require Import Coq.Classes.RelationClasses.
+
+
+Require Coq.Structures.Equalities Coq.Structures.EqualitiesFacts.
+Require Coq.Structures.Orders Coq.Structures.OrdersAlt Coq.Structures.OrdersFacts.
 
 Require Import  Coq.Classes.Morphisms_Prop.
 
 Import ListNotations.
 
-Inductive Card(Key Owner: Type) : Type :=
-| Talon: Key -> Card Key Owner
-| Assigned: Owner -> Card Key Owner.
+Import Coq.Structures.Equalities Coq.Structures.EqualitiesFacts.
+Import Coq.Structures.Orders Coq.Structures.OrdersAlt Coq.Structures.OrdersFacts.
+
+Require Import FunInd.
+
+Search nth.
+
+Module Card (Key Owner : DecidableType) <: DecidableType.
+  Inductive Card : Type :=
+  | Talon : Key.t -> Card
+  | Assigned : Owner.t -> Card.
+
+  Definition t := Card.
+
+  Definition eq : t -> t -> Prop :=
+    fun self other =>
+    match self, other with
+    | Talon self_key, Talon other_key => Key.eq self_key other_key
+    | Assigned self_owner, Assigned other_owner => Owner.eq self_owner other_owner
+    | _, _ => False
+    end.
+
+  Definition eq_talon_ind : forall (key : Key.t) (P : forall y : t, eq (Talon key) y -> Prop), (forall (y_key : Key.t) (x_eq_y : Key.eq key y_key), P (Talon y_key) x_eq_y) -> forall (y : t) (x_eq_y : eq (Talon key) y), P y x_eq_y.
+  Proof.
+    intros key P IHP [y_key| y_owner].
+      apply IHP.
+    contradiction.
+  Defined.
+
+  Definition eq_assigned_ind : forall (x_owner : Owner.t) (P : forall y : t, eq (Assigned x_owner) y -> Prop), (forall (y_owner : Owner.t) (x_eq_y : Owner.eq x_owner y_owner), P (Assigned y_owner) x_eq_y) -> forall (y : t) (x_eq_y : eq (Assigned x_owner) y), P y x_eq_y.
+  Proof.
+    intros x_owner P IHP [y_key| y_owner].
+      contradiction.
+    apply IHP.
+  Defined.
+
+  Instance eq_equiv : Equivalence eq.
+  Proof.
+    split.
+        intros card.
+        destruct card as [key| owner]; simpl; reflexivity.
+      intros [x_key| x_owner] [y_key| y_owner] x_eq_y; now simpl.
+    intros [x_key| x_owner] y z x_eq_y y_eq_z.
+      induction x_eq_y as [y_key x_eq_y] using eq_talon_ind.
+      induction y_eq_z as [z_key y_eq_z] using eq_talon_ind.
+      simpl.
+      now transitivity y_key.
+    induction x_eq_y as [y_key x_eq_y] using eq_assigned_ind.
+    induction y_eq_z as [z_key y_eq_z] using eq_assigned_ind.
+    simpl.
+    now transitivity y_key.
+  Defined.
+
+  Definition eq_dec : forall x y : t, {eq x y} + {~ eq x y}.
+  Proof.
+    intros x y.
+    destruct x as [x_key| x_owner], y as [y_key| y_owner].
+          apply Key.eq_dec.
+        now right.
+      now right.
+    apply Owner.eq_dec.
+  Defined.
+End Card.
+
+
+Module Option (E : DecidableType) <: DecidableType.
+  Definition t : Type := option E.t.
+
+  Definition eq : t -> t -> Prop :=
+    fun self other =>
+      match self, other with
+      | Some self_some, Some other_some => E.eq self_some other_some
+      | None, None => True
+      | _, _ => False
+      end.
+
+  Definition eq_None_ind : forall P : forall other : t, eq None other -> Prop, P None I -> forall (other : t) (self_eq_other : eq None other), P other self_eq_other.
+  Proof.
+    intros P P_None other self_eq_other.
+    destruct other as [other_some|].
+      contradiction.
+    now destruct self_eq_other.
+  Defined.
+
+  Definition eq_Some_ind : forall (self : E.t) (P : forall other : t, eq (Some self) other -> Prop), (forall (other : E.t) (self_eq_other : E.eq self other), P (Some other) self_eq_other) -> forall (other : t) (self_eq_other : eq (Some self) other), P other self_eq_other.
+Proof.
+    intros self P P_Some other self_eq_other.
+    destruct other as [other_some|].
+      now apply P_Some.
+    contradiction.
+  Defined.
+
+  Instance eq_equiv : Equivalence eq.
+  Proof.
+    split.
+        intros [x|]; simpl; reflexivity.
+      intros [x|] y x_eq_y.
+        induction x_eq_y as [y x_eq_y] using eq_Some_ind.
+        now simpl; symmetry.
+      now induction y, x_eq_y using eq_None_ind.
+    intros [x|] y z x_eq_y y_eq_z.
+      induction x_eq_y as [y x_eq_y] using eq_Some_ind.
+      induction y_eq_z as [z y_eq_z] using eq_Some_ind.
+      simpl.
+      now transitivity y.
+    induction y, x_eq_y using eq_None_ind.
+    induction z, y_eq_z using eq_None_ind.
+    easy.
+  Qed.
+
+  Definition eq_dec : forall x y : t, {eq x y} + {~ eq x y}.
+  Proof.
+    intros [x|] [y|].
+          apply E.eq_dec.
+        now right.
+      now right.
+    now left.
+  Defined.
+End Option.
 
 Module test (Key : OrderedType) (Owner: DecidableType).
 
-Module Positions (M: WSetsOn Owner).
 
-Definition positions: list (Card Key.t Owner.t) -> nat -> M.t.
+Module Import Card := Card Key Owner.
+Module Import OrderedFacts := OrderedTypeFacts Key.
+
+Module Talon.
+  Import Coq.FSets.FMapInterface Coq.FSets.FMapFacts.
+
+  Module Key' <: DecidableTypeOrig <: OrderedTypeOrig := Backport_OT Key.
+
+  Module Positions (M: Sfun Key').
+    Module Import MapFacts := WFacts_fun Key' M.
+
+Definition unwrap_or (A : Type) (self: option A) (default : A) : A :=
+  match self with
+  | Some x => x
+  | None => default
+  end.
+
+Module Interval.
+  Inductive t : Set :=
+  | new : nat -> nat -> t.
+
+  Definition singleton : nat -> t :=
+    fun n => new n n.
+
+  Definition lengthen : t -> nat -> t :=
+    fun interval right' =>
+      match interval with
+      | new l r => new l right'
+      end.
+
+  Definition left_endpoint : t -> nat :=
+    fun self => 
+      match self with
+      | new left_endpoint right_endpoint => left_endpoint
+      end.
+
+  Definition right_endpoint : t -> nat :=
+    fun self => 
+      match self with
+      | new left_endpoint right_endpoint => right_endpoint
+      end.
+End Interval.
+
+Function update (key_to_interval : M.t Interval.t) (key : Key.t) (index : nat) : M.t Interval.t :=
+  M.add key
+  (match M.find key key_to_interval with
+  | Some interval => Interval.lengthen interval index
+  | None => Interval.singleton index
+  end) key_to_interval.
+
+Function generate (cards : list Card.t) (index : nat) (key_to_interval : M.t Interval.t) : M.t Interval.t :=
+  match cards with
+  | [] => key_to_interval
+  | Talon head :: tail => generate tail (S index) (update key_to_interval head index)
+  | Assigned head :: tail => generate tail (S index) key_to_interval
+  end.
+
+  Definition generate_nil : forall (index : nat) (key_to_interval : M.t Interval.t), generate [] index key_to_interval = key_to_interval.
+  Proof.
+    reflexivity.
+  Defined.
+
+  Definition generate_cons_talon_MapsTo : forall (head : Key.t) (tail : list Card.t) (index : nat) (key_to_interval : M.t Interval.t) (interval : Interval.t), M.MapsTo head interval key_to_interval -> generate (Talon head :: tail) index key_to_interval = generate tail (S index) (M.add head (Interval.lengthen interval index) key_to_interval).
+  Proof.
+    intros head tail index key_to_interval interval head_MapsTo_interval.
+    simpl.
+    unfold update.
+    now rewrite M.find_1 with (1 := head_MapsTo_interval).
+  Defined.
+
+  Definition generate_cons_talon_not_In : forall (head : Key.t) (tail : list Card.t) (index : nat) (key_to_interval : M.t Interval.t), ~ M.In head key_to_interval -> generate (Talon head :: tail) index key_to_interval = generate tail (S index) (M.add head (Interval.singleton index) key_to_interval).
+  Proof.
+    intros head tail index key_to_interval not_In_head.
+    simpl.
+    unfold update.
+    replace (M.find head key_to_interval) with (@None Interval.t) by (symmetry; now apply not_find_in_iff).
+    reflexivity.
+  Defined.
+
+  Definition generate_cons_assigned : forall (head : Owner.t) (tail : list Card.t) (index : nat) (key_to_interval : M.t Interval.t), generate (Assigned head :: tail) index key_to_interval = generate tail (S index) key_to_interval.
+  Proof.
+    reflexivity.
+  Defined.
+
+  Definition MapsTo_dec : forall [elt : Type] (m : M.t elt) (x : M.key), {value : elt | M.MapsTo x value m} + ~ M.In x m.
+  Proof.
+    intros elt m x.
+    destruct (M.find x m) as [value|] eqn: test; [left| right].
+      exists value.
+      now apply M.find_2.
+    now apply not_find_in_iff.
+  Defined.
+
+
+Definition generate_ind' : forall (P : list Card.t -> nat -> M.t Interval.t -> M.t Interval.t -> Type), (forall (index : nat) (key_to_interval : M.t Interval.t), P [] index key_to_interval key_to_interval) -> (forall (head : Key.t) (tail : list Card.t) (index : nat) (key_to_interval : M.t Interval.t) (interval : Interval.t), M.MapsTo head interval key_to_interval -> P tail (S index) (M.add head (Interval.lengthen interval index) key_to_interval) (generate tail (S index) (M.add head (Interval.lengthen interval index) key_to_interval)) -> P  (Talon head :: tail) index key_to_interval (generate tail (S index) (M.add head (Interval.lengthen interval index) key_to_interval))) -> (forall (head : Key.t) (tail : list Card.t) (index : nat) (key_to_interval : M.t Interval.t), ~ M.In head key_to_interval -> P tail (S index) (M.add head (Interval.singleton index) key_to_interval) (generate tail (S index) (M.add head (Interval.singleton index) key_to_interval)) -> P (Talon head :: tail) index key_to_interval (generate tail (S index) (M.add head (Interval.singleton index) key_to_interval))) -> (forall (head : Owner.t) (tail : list Card.t) (index : nat) (key_to_interval : M.t Interval.t), P tail (S index) key_to_interval (generate tail (S index) key_to_interval) -> P (Assigned head :: tail) index key_to_interval (generate tail (S index) key_to_interval)) -> forall (cards : list Card.t) (index : nat) (key_to_interval : M.t Interval.t), P cards index key_to_interval (generate cards index key_to_interval).
+Proof.
+  intros P P_nil P_cons_talon_MapsTo P_cons_talon_not_In P_assigned .
+  simpl in *.
+  intros cards.
+  induction cards as [| [head| head] tail IHtail]; intros index key_to_interval.
+      apply P_nil.
+    specialize (IHtail (S index) (update key_to_interval head index)).
+    destruct (MapsTo_dec key_to_interval head) as [(interval & head_MapsTo_interval)| not_In_head].
+      rewrite generate_cons_talon_MapsTo with (1 := head_MapsTo_interval).
+      assert (update key_to_interval head index = M.add head (Interval.lengthen interval index) key_to_interval) as e.
+        unfold update.
+        now rewrite M.find_1 with (1 := head_MapsTo_interval).
+      rewrite e in IHtail.
+      now apply P_cons_talon_MapsTo.
+    rewrite generate_cons_talon_not_In with (1 := not_In_head).
+    assert (update key_to_interval head index = M.add head (Interval.singleton index) key_to_interval) as e.
+      unfold update.
+      replace (M.find head key_to_interval) with (@None Interval.t).
+        reflexivity.
+      symmetry; now apply not_find_in_iff.
+    rewrite e in IHtail.
+    simpl in *.
+    now apply P_cons_talon_not_In.
+  apply P_assigned.
+  specialize (IHtail (S index) key_to_interval).
+  apply IHtail.
+Defined.
+
+Definition generate_complete : forall (key : Key.t) (cards : list (Card.t)) (index : nat) (key_to_interval : M.t Interval.t), M.In key key_to_interval \/ InA Card.eq (Talon key) cards <-> M.In key (generate cards index key_to_interval).
+Proof.
+  intros key cards index key_to_interval.
+  functional induction (generate cards index key_to_interval) as [| ? index key_to_interval head tail ? IHtail| ? index key_to_interval head tail ? IHtail].
+      rewrite InA_nil.
+      firstorder.
+    rewrite InA_cons, <- IHtail.
+    cut (M.In key key_to_interval \/ eq (Talon key) (Talon head) <->
+M.In key (update key_to_interval head index)).
+      firstorder.
+    unfold update.
+    rewrite add_in_iff.
+    simpl.
+    assert (Key.eq key head <-> Key.eq head key) as -> by easy.
+    firstorder.
+  rewrite <- IHtail.
+  assert (InA eq (Talon key) (Assigned head :: tail) <-> InA eq (Talon key) tail) as ->.
+    rewrite InA_cons.
+    simpl.
+    firstorder.
+  firstorder.
+Defined.
+(*
+Definition generate_complete : forall (key : Key.t) (cards : list (Card.t)) (index : nat) (key_to_interval : M.t Interval.t), M.In key key_to_interval \/ InA Card.eq (Talon key) cards -> M.In key (generate cards index key_to_interval).
+Proof.
+  intros key cards index key_to_interval.
+  functional induction (generate cards index key_to_interval) as [| ? index key_to_interval head tail ? IHtail| ? index key_to_interval head tail ? IHtail]; intros In_key.
+      destruct In_key  as [In_key| In_key]; [assumption|].
+      now rewrite InA_nil in In_key.
+    destruct In_key as [In_key| In_key]; apply IHtail; [left|].
+      now apply add_in_iff; right.
+    apply InA_cons in In_key as [key_eq_head| In_key]; [left| right].
+      unfold update.
+      now apply add_in_iff; left.
+    assumption.
+  destruct In_key as [In_key| In_key]; apply IHtail; [left| right].
+    assumption.
+  apply InA_cons in In_key as [key_eq_head| In_key].
+    contradiction.
+  assumption.
+Defined.
+*)
+Module Option := Option Card.
+
+Definition generate_left_const : forall (key : Key.t) (cards : list (Card.t)) (index : nat) (key_to_interval : M.t Interval.t) (interval : Interval.t), M.MapsTo key interval key_to_interval -> exists right_endpoint : nat, M.MapsTo key (Interval.new (Interval.left_endpoint interval) right_endpoint) (generate cards index key_to_interval).
+Proof.
+  intros key cards index key_to_interval.
+  functional induction (generate cards index key_to_interval) as [| ? index key_to_interval head tail ? IHtail| ? index key_to_interval head tail ? IHtail]; intros interval MapsTo_key_interval.
+      destruct interval as [left_endpoint right_endpoint].
+      now exists right_endpoint.
+    destruct (Key.eq_dec head key) as [head_eq_key| head_neq_key].
+      assert (M.MapsTo key (Interval.lengthen interval index) (update key_to_interval head index)) as H.
+        unfold update.
+        rewrite M.find_1 with (e := interval).
+          now apply M.add_1.
+        now rewrite head_eq_key.
+      destruct IHtail with (1 := H) as [right_endpoint H'].
+      destruct interval as [left_endpoint' right_endpoint'].
+      simpl in *.
+      exists right_endpoint.
+      assumption.
+    now apply IHtail, M.add_2.
+  now apply IHtail.
+Defined.
+
+Definition generate_right_const : forall (key : Key.t) (cards : list (Card.t)) (index : nat) (key_to_interval : M.t Interval.t), ~ InA Card.eq (Talon key) cards -> option_map Interval.right_endpoint (M.find key key_to_interval) = option_map Interval.right_endpoint (M.find key (generate cards index key_to_interval)).
+Proof.
+  intros key cards index key_to_interval.
+  functional induction (generate cards index key_to_interval) as [| ? index key_to_interval head tail ? IHtail| ? index key_to_interval head tail ? IHtail]; intros not_In_key.
+      reflexivity.
+    assert (~ Key.eq key head /\ ~ InA Card.eq (Talon key) tail) as [key_neq_head not_In_key_tail].
+      cut (~ (Key.eq key head \/ InA eq (Talon key) tail)).
+        auto.
+      contradict not_In_key.
+      now apply InA_cons.
+    rewrite <- IHtail with (1 := not_In_key_tail).
+    unfold update.
+    now rewrite add_neq_o; [| contradict key_neq_head].
+  apply IHtail.
+  contradict not_In_key.
+  now constructor 2.
+Defined.
+
+
+Definition generate_left_new : forall (key : Key.t) (cards : list (Card.t)) (index : nat) (key_to_interval : M.t Interval.t), ~ M.In key key_to_interval -> forall interval : Interval.t, M.MapsTo key interval (generate cards index key_to_interval) -> exists offset : nat, Interval.left_endpoint interval = index + offset /\ (forall n : nat, n < offset -> ~ Option.eq (nth_error cards n) (Some (Talon key))) /\ Option.eq (nth_error cards offset) (Some (Talon key)).
+Proof.
+  intros key cards index key_to_interval.
+  functional induction (generate cards index key_to_interval) as [| ? index key_to_interval head tail ? IHtail| ? index key_to_interval head tail ? IHtail]; intros not_In_key interval MapsTo_key_interval.
+      contradict not_In_key.
+      now exists interval.
+    destruct (Key.eq_dec head key) as [head_eq_key| head_neq_key].
+      exists 0.
+      repeat split.
+          rewrite PeanoNat.Nat.add_0_r.
+          assert (M.MapsTo key (Interval.singleton index) (update key_to_interval head index)).
+            unfold update.
+            rewrite head_eq_key.
+            replace (M.find key key_to_interval) with (@None Interval.t).
+              now apply M.add_1.
+            symmetry.
+            now apply not_find_in_iff.
+          destruct (@generate_left_const key tail (S index) _ _ H) as [right_endpoint H'].
+          replace interval with (Interval.new index right_endpoint).
+            reflexivity.
+          now apply MapsTo_fun with (1 := H').
+        intros n n_lt_0.
+        contradict n_lt_0.
+        apply PeanoNat.Nat.nlt_0_r.
+      assumption.
+    assert (~ M.In key (update key_to_interval head index)) as H.
+      unfold update.
+      now rewrite add_neq_in_iff.
+    specialize (IHtail H interval MapsTo_key_interval).
+    destruct IHtail as [offset (H₁ & H₂ & H₃)].
+    exists (S offset).
+    repeat split.
+        now rewrite PeanoNat.Nat.add_succ_r.
+      destruct n as [| n].
+        easy.
+      intros n_lt_offset.
+      now apply H₂, Lt.lt_S_n.
+    assumption.
+  specialize (IHtail not_In_key interval MapsTo_key_interval).
+  destruct IHtail as [offset (H₁ & H₂ & H₃)].
+  exists (S offset).
+  repeat split.
+      now rewrite PeanoNat.Nat.add_succ_r.
+    destruct n as [| n].
+      easy.
+    intros n_lt_offset.
+    now apply H₂, Lt.lt_S_n.
+  assumption.
+Defined.
+
+Functional Scheme nth_error_ind := Induction for nth_error Sort Prop.
+
+Definition nth_error_InA : forall (key : Key.t) (index : nat) (cards : list Card.t), Option.eq (nth_error cards index) (Some (Talon key)) -> InA Card.eq (Talon key) cards.
+Proof.
+  intros key index.
+  induction index as [| index' IHindex']; intros [| head tail] H; try contradiction.
+    now constructor 1.
+  now constructor 2; apply IHindex'.
+Defined.
+
+Definition generate_right_new : forall (key : Key.t) (cards : list (Card.t)) (index : nat) (key_to_interval : M.t Interval.t), InA Card.eq (Talon key) cards -> forall interval : Interval.t, M.MapsTo key interval (generate cards index key_to_interval) -> exists offset : nat, Interval.right_endpoint interval = index + offset /\ (forall n : nat, n > offset -> ~ Option.eq (nth_error cards n) (Some (Talon key))) /\ Option.eq (nth_error cards offset) (Some (Talon key)).
+Proof.
+  intros key cards index key_to_interval.
+  functional induction (generate cards index key_to_interval) as [| ? index key_to_interval head tail ? IHtail| ? index key_to_interval head tail ? IHtail]; intros In_key_cards interval MapsTo_key_interval.
+      now apply InA_nil in In_key_cards.
+    destruct (InA_dec Card.eq_dec (Talon key) tail) as [In_key_tail| not_In_key_tail].
+      destruct IHtail with (1 := In_key_tail) (2 := MapsTo_key_interval) as [offset (H₁ & H₂ & H₃)].
+      exists (S offset).
+      repeat split.
+          now rewrite PeanoNat.Nat.add_succ_r.
+        destruct n as [| n].
+          easy.
+        intros n_lt_offset.
+        now apply H₂, Lt.lt_S_n.
+      assumption.
+    assert (Key.eq key head) as key_eq_head by now apply InA_cons in In_key_cards as [key_eq_head| In_key_tail].
+    exists 0.
+    repeat split.
+        rewrite PeanoNat.Nat.add_0_r.
+        pose (H := generate_right_const (S index) (update key_to_interval head index) not_In_key_tail).
+        cut (Some (Interval.right_endpoint interval) = Some index).
+          now inversion 1.
+        transitivity (option_map Interval.right_endpoint (M.find key (generate tail (S index) (update key_to_interval head index)))).
+          now rewrite M.find_1 with (1 := MapsTo_key_interval).
+        transitivity (option_map Interval.right_endpoint (M.find key (update key_to_interval head index))).
+          easy.
+        unfold update.
+        rewrite add_eq_o by easy.
+        now destruct (M.find head key_to_interval) as [[left_endpoint right_endpoint]|].
+      intros [| n'] n_gt_0.
+        contradict n_gt_0.
+        apply PeanoNat.Nat.lt_irrefl.
+      simpl.
+      contradict not_In_key_tail.
+      now apply nth_error_InA with n'.
+    easy.
+  assert (InA Card.eq (Talon key) tail) as In_key_tail by now apply InA_cons in In_key_cards as [key_eq_head| In_key_tail].
+  destruct IHtail with (1 := In_key_tail) (2 := MapsTo_key_interval) as [offset (H₁ & H₂ & H₃)].
+  exists (S offset).
+  repeat split.
+      now rewrite PeanoNat.Nat.add_succ_r.
+    destruct n as [| n].
+      easy.
+    intros n_lt_offset.
+    now apply H₂, Lt.lt_S_n.
+  assumption.
+Defined.
+
+
+(*
+Definition generate_lol : forall (cards : list (Card.t)) (index : nat) (key_to_interval : M.t Interval.t) (key : Key.t), ~ M.In key key_to_interval -> forall interval : Interval.t, M.MapsTo key interval (generate cards index key_to_interval) -> exists n : nat, Interval.left_endpoint interval = n + index /\ Option.eq (nth_error cards n) (Some (Talon key)).
 Proof.
   intros cards.
-  induction cards as [| [key| owner] tail IHtail]; intros index.
-Admitted.
+  induction cards as [| [head| head] tail IHtail]; intros index key_to_interval key not_In_key_intervals interval MapsTo_key_interval.
+      assert (M.In key key_to_interval) by now exists interval.
+      contradiction.
+    specialize (IHtail (S index) (update key_to_interval head index) key).
+    destruct (Key.eq_dec head key) as [head_eq_key| head_neq_key].
+      simpl in *.
+      unfold update in *.
+      simpl in *.
+      replace (M.find head key_to_interval) with (@None Interval.t) in MapsTo_key_interval.
+        assert (M.MapsTo key (Interval.singleton index) (M.add head (Interval.singleton index) key_to_interval)) as H.
+          now apply M.add_1.
+        destruct (@generate_left_endpoint tail (S index) (M.add head (Interval.singleton index) key_to_interval) key (Interval.singleton index) H) as [right_endpoint H'].
+        Search (M.MapsTo _ _ _ -> _ = _).
+        simpl in *.
+        assert (interval = Interval.new index right_endpoint) as ->.
+          now apply MapsTo_fun with (1 := MapsTo_key_interval).
+        simpl.
+        exists 0.
+        split.
+          reflexivity.
+        assumption.
+      symmetry.
+      apply not_find_in_iff.
+      now rewrite head_eq_key.
+    assert (~ M.In key (update key_to_interval head index)) as not_In_key_update.
+      intros In_key_update.
+      apply add_neq_in_iff in In_key_update.
+        contradiction.
+      assumption.
+    specialize (IHtail not_In_key_update interval MapsTo_key_interval).
+    destruct IHtail as [n [H₁ H₂]].
+    exists (S n).
+    split.
+      now rewrite PeanoNat.Nat.add_succ_r in H₁.
+    assumption.
+  specialize (IHtail (S index) key_to_interval key not_In_key_intervals interval MapsTo_key_interval).
+  destruct IHtail as [n [H₁ H₂]].
+  exists (S n).
+  split.
+    now rewrite PeanoNat.Nat.add_succ_r in H₁.
+  assumption.
+Defined.
+*)
+(*
+Definition generate_not_in : forall (cards : list (Card.t)) (index : nat) (key_to_interval : M.t Interval.t) (key : Key.t), ~ Exists (card_eq (Talon _ key)) cards -> forall interval : Interval.t, M.MapsTo key interval (generate cards index key_to_interval) <-> M.MapsTo key interval key_to_interval.
+Proof.
+  intros cards.
+  induction cards as [| head tail IHtail]; intros index key_to_interval key not_In_key_cards interval.
+    reflexivity.
+  assert (~ Exists (card_eq (Talon Owner.t key)) tail) as not_In_key_tail.
+    contradict not_In_key_cards.
+    now constructor 2.
+  assert (~ card_eq (Talon Owner.t key) head) as key_neq_head.
+    contradict not_In_key_cards.
+    now constructor 1.
+  destruct head as [head| head].
+    simpl in *.
+    specialize (IHtail (S index) (update key_to_interval head index) key not_In_key_tail interval).
+    assert (M.MapsTo key interval (update key_to_interval head index) <-> M.MapsTo key interval key_to_interval) as H.
+      unfold update.
+      rewrite add_neq_mapsto_iff.
+        reflexivity.
+      now contradict key_neq_head.
+    now rewrite H in IHtail.
+  now apply IHtail.
+Defined.
 
+Definition generate_lol_final : forall (cards : list (Card.t)) (index : nat) (key_to_interval : M.t Interval.t) (key : Key.t), Exists (card_eq (Talon _ key)) cards -> forall interval : Interval.t, M.MapsTo key interval (generate cards index key_to_interval) -> exists n : nat, Interval.right_endpoint interval = n + index /\ option_eq card_eq (nth_error cards n) (Some (Talon _ key)).
+Proof.
+  intros cards.
+  induction cards as [| [head| head] tail IHtail]; intros index key_to_interval key In_key_cards interval MapsTo.
+      now rewrite Exists_nil in In_key_cards.
+    specialize (IHtail (S index) (update key_to_interval head index) key).
+    destruct (Exists_dec _ tail (@card_eq_dec (Talon _ key))) as [In_key_tail| not_In_key_tail].
+      specialize (IHtail In_key_tail _ MapsTo).
+      destruct IHtail as [n [H₁ H₂]].
+      exists (S n).
+      split.
+        now rewrite PeanoNat.Nat.add_succ_r in H₁.
+      assumption.
+    apply Exists_cons in In_key_cards as [key_eq_head| In_key_tail].
+      simpl in key_eq_head.
+      simpl in MapsTo.
+      rewrite generate_not_in in MapsTo by assumption.
+      unfold update in *.
+      Search (M.MapsTo _ _ (M.add _ _ _)).
+      rewrite add_mapsto_iff in MapsTo.
+      destruct MapsTo as [[_ e]| [? ?]].
+        rewrite <- e.
+        replace (  Interval.right_endpoint
+    match M.find head key_to_interval with
+    | Some interval0 => Interval.lengthen interval0 index
+    | None => Interval.singleton index
+    end) with index.
+          exists 0.
+          split.
+            reflexivity.
+          simpl.
+          now symmetry.
+        now destruct (M.find head key_to_interval) as [[? ?]|]; simpl.
+      now contradict H.
+    contradiction.
+  apply Exists_cons in In_key_cards as [key_eq_head| In_key_tail].
+    contradiction.
+  specialize (IHtail (S index) key_to_interval key In_key_tail interval MapsTo).
+  destruct IHtail as (n & [H₁ H₂]).
+  exists (S n).
+  split.
+    now rewrite PeanoNat.Nat.add_succ_r in H₁.
+  assumption.
+Defined.
+*)
+Definition intervals : list (Card.t) -> M.t Interval.t :=
+  fun cards => generate cards 0 (M.empty _).
+
+Definition intervals_complete : forall (cards : list (Card.t)) (key : Key.t), InA Card.eq (Talon key) cards -> M.In key (intervals cards).
+Proof.
+  intros cards key In_key_cards.
+  apply generate_complete.
+  now right.
+Defined.
+
+Definition intervals_correct : forall (cards : list Card.t) (key : Key.t) (interval : Interval.t), M.MapsTo key interval (intervals cards) -> (forall n : nat, n < (Interval.left_endpoint interval) -> ~ Option.eq (nth_error cards n) (Some (Talon key))) /\ Option.eq (nth_error cards (Interval.left_endpoint interval)) (Some (Talon key)) /\  Option.eq (nth_error cards (Interval.right_endpoint interval)) (Some (Talon key)) /\ (forall n : nat, n > (Interval.right_endpoint interval) -> ~ Option.eq (nth_error cards n) (Some (Talon key))).
+Proof.
+  intros cards key interval MapsTo_key_interval.
+  assert (M.In key (intervals cards)) as In_key by now exists interval.
+  assert (InA Card.eq (Talon key) cards) as In_key_cards.
+    apply generate_complete in In_key.
+    rewrite empty_in_iff in In_key.
+    firstorder.
+  assert (~ M.In key (M.empty Interval.t)) as not_In_key by now rewrite empty_in_iff.
+  destruct generate_left_new with (1 := not_In_key) (2 := MapsTo_key_interval) as [left_endpoint (left_H₁ & left_H₂ & left_H₃)].
+  destruct generate_right_new with (1 := In_key_cards) (2 := MapsTo_key_interval) as [right_endpoint (right_H₁ & right_H₂ & right_H₃)].
+  rewrite right_H₁, left_H₁.
+  simpl.
+  repeat split; try assumption.
+Defined.
+(*
+Definition intervals_correct_iff : forall (cards : list Card.t) (key : Key.t) (interval : Interval.t), M.MapsTo key interval (intervals cards) <-> (forall n : nat, n < (Interval.left_endpoint interval) -> ~ Option.eq (nth_error cards n) (Some (Talon key))) /\ Option.eq (nth_error cards (Interval.left_endpoint interval)) (Some (Talon key)) /\  Option.eq (nth_error cards (Interval.right_endpoint interval)) (Some (Talon key)) /\ (forall n : nat, n > (Interval.right_endpoint interval) -> ~ Option.eq (nth_error cards n) (Some (Talon key))).
+Proof.
+  intros cards key interval.
+  split.
+    apply intervals_correct.
+  destruct 1 as (H₂_left & H₃_left & H₂_right & H₃_right).
+Admitted.*)
 End Positions.
 
+Import Coq.MSets.MSetFacts Coq.MSets.MSetProperties.
 
 Module Owners (M : WSetsOn Owner).
 
 Module Import Facts := WFactsOn Owner M.
 Module Import Properties := WPropertiesOn Owner M.
 
-Definition owners_helper : list (Card Key.t Owner.t) -> M.t -> list Owner.t.
+Definition owners_helper : list (Card.t) -> M.t -> list Owner.t.
 Proof.
   intros cards.
   induction cards as [| [key| owner] tail IHtail]; intros seen.
@@ -40,10 +623,10 @@ Proof.
   exact (if M.mem owner seen then IHtail seen else owner:: IHtail (M.add owner seen)).
 Defined.
 
-Definition owners: list (Card Key.t Owner.t) ->list Owner.t :=
+Definition owners: list (Card.t) ->list Owner.t :=
 fun cards => owners_helper cards M.empty.
 
-Definition owners_subset : forall (cards: list (Card Key.t Owner.t)) (seen seen' : M.t), M.Subset seen seen' -> forall owner, In owner (owners_helper cards seen') -> In owner (owners_helper cards seen).
+Definition owners_subset : forall (cards: list (Card.t)) (seen seen' : M.t), M.Subset seen seen' -> forall owner, Exists (Owner.eq owner) (owners_helper cards seen') -> Exists (Owner.eq owner) (owners_helper cards seen).
 Proof.
   intros cards.
   induction cards as [| [head_key| head_owner] tail IHtail]; intros seen seen' seen_le_seen' owner.
@@ -66,6 +649,7 @@ Proof.
     assumption.
   simpl.
   intros H.
+  apply Exists_cons in H.
   destruct H.
     now left.
   right.
@@ -75,16 +659,17 @@ Proof.
   assumption.
 Defined.
 
-
-Definition helper_complete : forall (cards: list (Card Key.t Owner.t)) (seen: M.t) (owner : Owner.t), ~ M.In owner seen -> In owner (owners_helper cards seen) <-> In (Assigned Key.t owner) cards.
+Definition helper_complete : forall (cards: list (Card.t)) (seen: M.t) (owner : Owner.t), ~ M.In owner seen -> Exists (Owner.eq owner) (owners_helper cards seen) <-> Exists (Card.eq (Assigned owner)) cards.
 Proof.
   induction cards as [| [head_key| head_owner] tail IHtail]; intros seen owner In_owner_seen.
-      reflexivity.
+      now rewrite ?Exists_nil.
     simpl.
-    assert (In (Assigned Key.t owner) (Talon Owner.t head_key :: tail) <-> In (Assigned Key.t owner) tail) as ->.
+    assert (Exists (Card.eq (Assigned owner)) (Talon head_key :: tail) <-> Exists (Card.eq (Assigned owner)) tail) as ->.
       split.
-        destruct 1 as [owner_eq_head| In_owner_tail].
-          discriminate owner_eq_head.
+        intros H.
+        apply Exists_cons in H.
+        destruct H as [owner_eq_head| In_owner_tail].
+          contradiction.
         assumption.
       intros In_owner_tail.
       now right.
@@ -96,20 +681,23 @@ Proof.
       right.
       now apply IHtail with seen.
     simpl.
-    destruct 1 as [->| In_owner_tail].
-      left.
-      now f_equal.
+    intros H.
+    apply Exists_cons in H.
+    destruct H as [e| In_owner_tail].
+      now left.
     destruct (Owner.eq_dec owner head_owner).
-      left.
-      admit.
+      now left.
     right.
     apply IHtail with (seen := seen).
       assumption.
     apply owners_subset with (seen' := (M.add head_owner seen)).
       now apply subset_add_2.
     assumption.
-  destruct 1 as [head_owner_eq_owner| In_owner_tail].
-    injection head_owner_eq_owner as ->.
+  intros H.
+  apply Exists_cons in H.
+  destruct H as [head_owner_eq_owner| In_owner_tail].
+    simpl in head_owner_eq_owner.
+    rewrite <- head_owner_eq_owner.
     destruct (M.mem owner seen) eqn: mem_owner_seen.
       now rewrite M.mem_spec in mem_owner_seen.
     now left.
@@ -119,27 +707,25 @@ Proof.
   (*specialize (IHtail seen owner In_owner_seen).*)
   destruct (Owner.eq_dec owner head_owner) as [owner_eq_head_owner| owner_neq_head_owner].
     left.
-    admit.
+    assumption.
   right.
-  assert (In owner (owners_helper tail seen)).
+  assert (Exists (Owner.eq owner) (owners_helper tail seen)).
     now rewrite IHtail.
   rewrite (IHtail (M.add head_owner seen) owner).
     assumption.
   intros H'.
   rewrite M.add_spec in H'.
   destruct H' as [owner_eq_head_owner| In_owner_seen'].
-    admit.
-  admit.
-Admitted.
-
-Definition complete : forall (cards: list (Card Key.t Owner.t))(owner : Owner.t), In owner (owners cards) <-> In (Assigned Key.t owner) cards.
-Admitted.
-
+    contradiction.
+  contradiction.
+Defined.
 
 End Owners.
 
 
-Definition owners : list (Card Key.t Owner.t) -> list Owner.t.
+
+
+Definition owners : list (Card.t) -> list Owner.t.
 Proof.
   intros cards.
   induction cards as [| head tail IHtail].
@@ -149,6 +735,6 @@ Proof.
   exact (owner :: IHtail).
 Defined.
 
+End Talon.
 End test.
-
 
